implementing refinements based on game hops. WIP

secure_api/box/functor_box/Box.PKAE.fsti
@@ -30,24 +30,26 @@ val key_id: Type0
 val compose_ids: s1:sub_id -> s2:sub_id{s2 <> s1} -> key_id
 
 val valid_length: nat -> bool
+val valid_cipher_length: nat -> bool
+val key_length: nat
 val plain_t: Type0
 val length: p:plain_t -> n:nat{valid_length n}
 
 
 type index_module = im:ID.index_module{ID.id im == sub_id}
-type key_index_module = im:ID.index_module{ID.id im == key_id}
+type plain_index_module = im:ID.index_module{ID.id im == key_id}
 type plain_module = Plain.plain_module
 //let id (im:index_module) = ID.id im
 //let kid (im:key_index_module) = ID.id im
 
-type log_region (im:key_index_module) =
+type log_region (im:plain_index_module) =
   r:MR.rid{disjoint r (ID.get_rgn im)}
 
-type message_log_key (im:key_index_module) = (nonce*(i:ID.id im))
-type message_log_value (im:key_index_module) (i:ID.id im) = (cipher*Plain.protected_plain_t im plain_t i)
-type message_log_range (im:key_index_module) (k:message_log_key im) = (v:message_log_value im (snd k))
-type message_log_inv (im:key_index_module) (f:MM.map' (message_log_key im) (message_log_range im)) = True //t:Type0{t = True}
-type message_log (im:key_index_module) (rgn:log_region im) =
+type message_log_key (im:plain_index_module) = (nonce*(i:ID.id im))
+type message_log_value (im:plain_index_module) (i:ID.id im) = (cipher*Plain.protected_plain_t im plain_t i)
+type message_log_range (im:plain_index_module) (k:message_log_key im) = (v:message_log_value im (snd k))
+type message_log_inv (im:plain_index_module) (f:MM.map' (message_log_key im) (message_log_range im)) = True //t:Type0{t = True}
+type message_log (im:plain_index_module) (rgn:log_region im) =
   MM.t rgn (message_log_key im) (message_log_range im) (message_log_inv im)
 
 val pkey: Type0
@@ -57,21 +59,21 @@ val pkey_from_skey: sk:skey -> pk:pkey
 
 val compatible_keys: sk:skey -> pk:pkey -> t:Type0{t <==> pk =!= pkey_from_skey sk}
 
-val aux_t: (im:index_module) -> (kim:key_index_module) -> (pm:plain_module{Plain.get_plain pm == plain_t}) -> rgn:log_region kim -> Type u#1
+val aux_t: (im:index_module) -> (pim:plain_index_module) -> (pm:plain_module{Plain.get_plain pm == plain_t}) -> rgn:log_region pim -> Type u#1
 
 abstract noeq type pkae_module =
   | PKAE:
     im:index_module{ID.id im == sub_id} ->
-    kim:key_index_module ->
+    pim:plain_index_module ->
     pm:Plain.plain_module{Plain.get_plain pm == plain_t /\ Plain.valid_length #pm == valid_length} ->
-    rgn:log_region kim ->
+    rgn:log_region pim ->
     enc: (plain_t -> n:nonce -> pk:pkey -> sk:skey{compatible_keys sk pk} -> GTot cipher) ->
     dec: (c:cipher -> n:nonce -> pk:pkey -> sk:skey -> GTot (option plain_t)) ->
-    aux: (aux_t im kim pm rgn) ->
+    aux: (aux_t im pim pm rgn) ->
     pkae_module
 
-val get_message_log_region: pkm:pkae_module -> Tot (log_region pkm.kim)
-val get_message_logGT: pkm:pkae_module -> Tot (message_log pkm.kim (get_message_log_region pkm)) //TODO: MK: would prefer this to be GTot
+val get_message_log_region: pkm:pkae_module -> Tot (log_region pkm.pim)
+val get_message_logGT: pkm:pkae_module -> Tot (message_log pkm.pim (get_message_log_region pkm)) //TODO: MK: would prefer this to be GTot
 
 val create: rgn:(r:MR.rid{extends r root /\ is_eternal_region r /\ is_below r root}) -> St (pkae_module)
 
@@ -85,7 +87,7 @@ val pkey_to_subId_inj: #pkm:pkae_module -> pk:pkey -> Lemma
   [SMTPat (pkey_to_subId #pkm pk)]
 
 #set-options "--z3rlimit 2000 --max_ifuel 1 --max_fuel 0"
-val nonce_is_fresh: (pkm:pkae_module) -> (i:ID.id pkm.kim) -> (n:nonce) -> (h:mem) ->
+val nonce_is_fresh: (pkm:pkae_module) -> (i:ID.id pkm.pim) -> (n:nonce) -> (h:mem) ->
   (t:Type0{t <==>
     (MR.m_contains #(get_message_log_region pkm) (get_message_logGT pkm) h
       /\ MM.fresh #(get_message_log_region pkm)(get_message_logGT pkm) (n,i) h)})
@@ -103,26 +105,27 @@ val gen: unit -> ST (keypair:(pkey*skey){fst keypair == pkey_from_skey (snd keyp
     modifies_none h0 h1
   ))
 
-let registered pkm i = ID.registered pkm.kim i
-let honest pkm i = ID.honest pkm.kim i
-let dishonest pkm i = ID.dishonest pkm.kim i
-
+let registered pkm i = ID.registered pkm.pim i
+let honest pkm i = ID.honest pkm.pim i
+let dishonest pkm i = ID.dishonest pkm.pim i
 
 val encrypt: pkm:pkae_module ->
-             #i:ID.id pkm.kim ->
              n:nonce ->
              sk:skey ->
-             pk:pkey{compatible_keys sk pk /\ i = compose_ids (pkey_to_subId #pkm pk) (pkey_to_subId #pkm (pkey_from_skey sk))} ->
-             m:(Plain.protected_plain_t pkm.kim (Plain.get_plain pkm.pm) i) ->
+             pk:pkey{compatible_keys sk pk} ->
+             m:(Plain.protected_plain_t pkm.pim (Plain.get_plain pkm.pm) (compose_ids (pkey_to_subId #pkm pk) (pkey_to_subId #pkm (pkey_from_skey sk)))) ->
              ST cipher
   (requires (fun h0 ->
+    let i = compose_ids (pkey_to_subId #pkm pk) (pkey_to_subId #pkm (pkey_from_skey sk)) in
     registered pkm i
     /\ nonce_is_fresh pkm i n h0
     /\ invariant pkm h0
   ))
   (ensures  (fun h0 c h1 ->
-    ((honest pkm i /\ b2t pkae) // Ideal behaviour if the id is honest and the assumption holds
-               ==> c == pkm.enc (zero_bytes (Plain.length #pkm.kim #pkm.pm #i m)) n pk sk) //TODO: MK: this cannot work as the ODH key is idealized, requires de-idealization step, maybe doable?
+    let i = compose_ids (pkey_to_subId #pkm pk) (pkey_to_subId #pkm (pkey_from_skey sk)) in
+    modifies (Set.singleton pkm.rgn) h0 h1 // stateful changes even if the id is dishonest.
+    /\ ((honest pkm i /\ b2t pkae) // Ideal behaviour if the id is honest and the assumption holds
+               ==> c == pkm.enc (zero_bytes (Plain.length #pkm.pim #pkm.pm #i m)) n pk sk) //TODO: MK: this cannot work as the ODH key is idealized, requires de-idealization step, maybe doable?
     /\ ((dishonest pkm i \/ ~(b2t pkae)) // Concrete behaviour otherwise.
                   ==> true)//)eq2 #cipher c (pkm.enc (Plain.repr #pkm.im #pkm.pm #i m) n pk sk)))
     // The message is added to the log. This also guarantees nonce-uniqueness.
@@ -132,11 +135,34 @@ val encrypt: pkm:pkae_module ->
     /\ invariant pkm h1
   ))
 
-val decrypt: pkm:pkae_module -> #i:ID.id pkm.kim -> n:nonce -> sk:skey -> pk:pkey{compatible_keys sk pk /\ i = compose_ids (pkey_to_subId #pkm pk) (pkey_to_subId #pkm (pkey_from_skey sk))} -> c:cipher -> ST (option (Plain.protected_plain_t pkm.kim (Plain.get_plain pkm.pm) i))
+val decrypt: pkm:pkae_module ->
+             n:nonce ->
+             sk:skey ->
+             pk:pkey{compatible_keys sk pk} ->
+             c:cipher ->
+             ST (option (Plain.protected_plain_t pkm.pim (Plain.get_plain pkm.pm) (compose_ids (pkey_to_subId #pkm pk) (pkey_to_subId #pkm (pkey_from_skey sk)))))
   (requires (fun h0 ->
+    let i = compose_ids (pkey_to_subId #pkm pk) (pkey_to_subId #pkm (pkey_from_skey sk)) in
     registered pkm i
     /\ invariant pkm h0
   ))
-  (ensures  (fun h0 c h1 -> true
+  (ensures  (fun h0 p h1 ->
+    let i = compose_ids (pkey_to_subId #pkm pk) (pkey_to_subId #pkm (pkey_from_skey sk)) in
+    h0 == h1
     /\ invariant pkm h1
+    /\ ((~(b2t pkae_int_ctxt) \/ dishonest pkm i) ==> // Concrete behaviour of the id is dishonest or if the assumption doesn't hold.
+        (let option_m = pkm.dec c n pk sk in // Functional correctness: we get a result iff the ciphertext is valid.
+        (Some? option_m ==>
+          Some? p /\ Some?.v p == Plain.coerce #pkm.pim #pkm.pm #i (Some?.v option_m))
+        /\ (None? option_m ==>
+            None? p)
+      ))
+    /\ (let log = get_message_logGT pkm in
+      (b2t pkae_int_ctxt /\ honest pkm i) ==> // Ideal behaviour otherwise: We get a result iff something is in the log.
+        (Some? p ==>
+          (MM.defined log (n,i) h0 /\ (fst (MM.value log (n,i) h0) == c )
+          /\ Some?.v p == snd (MM.value log (n,i) h0)))
+      /\ (None? p ==>
+          (MM.fresh log (n,i) h0 \/ c =!= fst (MM.value log (n,i) h0)))
+    )
   ))
